src/dafny/smart/Helpers.dfy
@@ -1,0 +1,37 @@
+/*
+ * Copyright 2020 ConsenSys AG.
+ *
+ * Licensed under the Apache License, Version 2.0 (the "License"); you may 
+ * not use this file except in compliance with the License. You may obtain 
+ * a copy of the License at http://www.apache.org/licenses/LICENSE-2.0
+ *
+ * Unless required by applicable law or agreed to in writing, software dis-
+ * tributed under the License is distributed on an "AS IS" BASIS, WITHOUT 
+ * WARRANTIES OR CONDITIONS OF ANY KIND, either express or implied. See the 
+ * License for the specific language governing permissions and limitations 
+ * under the License.
+ */
+ 
+module Helpers {
+
+    /**
+     *  Maximum of two non-negative integers.
+     */
+    function max(x: nat, y : nat) : nat 
+    {
+        if x > y then 
+            x
+        else 
+            y
+    }
+
+    /** Define 2^n. */
+    function power2(n : nat): nat 
+        ensures power2(n) >= 1
+        ensures n >= 1 ==> power2(n) >= 2 
+
+        decreases n
+    {
+        if n == 0 then 1 else 2 * power2(n - 1)
+    }
+}
